Introduce well formed traces

rupicola/io/Hist.fst
@@ -2,7 +2,7 @@ module Hist
 
 open FStar.Tactics
 open FStar.List.Tot.Base
-
+open Trace
 (** The postcondition for an io computation is defined over the
 result (type: a) and local trace (type: list event).
 The local trace represents the events that happend during the
@@ -15,90 +15,92 @@ The history is in reverse chronological order.
 At the end of an io computation, the local trace is
 reversed and appended to the history. **)
 
-let hist_post (#event_type:Type) a = lt:list event_type -> r:a -> Type0
-let hist_pre (#event_type:Type) = h:list event_type -> Type0
+let hist_post (h:history) a = lt:local_trace h -> r:a -> Type0
+let hist_pre = h:history -> Type0
 
-type hist0 (#event_type:Type) a = hist_post #event_type a -> hist_pre #event_type
-
-unfold
-let hist_post_ord (#event_type:Type) (p1 p2:hist_post #event_type 'a) = forall lt r. p1 lt r ==> p2 lt r
+type hist0 a =
+  h:history -> hist_post h a -> Type0
 
 unfold
-let hist_wp_monotonic (#event_type:Type) (wp:hist0 #event_type 'a) =
-  forall p1 p2. (p1 `hist_post_ord` p2) ==> (forall h. wp p1 h ==> wp p2 h)
+let hist_post_ord (#h:history) (p1 p2:hist_post h 'a) = forall lt r. p1 lt r ==> p2 lt r
 
-type hist #event_type a = wp:(hist0 #event_type a){hist_wp_monotonic wp}
+unfold
+let hist_wp_monotonic (wp:hist0 'a) =
+  forall h (p1 p2:hist_post h 'a). (p1 `hist_post_ord` p2) ==>  (wp h p1 ==> wp h p2)
 
-val hist_subcomp0 : #event_type:Type -> #a:Type -> #p1:(a -> Type0) -> #p2:(a -> Type0) -> #_:unit{forall x. p1 x ==> p2 x} -> wp:hist #event_type (x:a{p1 x}) -> 
-  (hist #event_type (x:a{p2 x}))
-let hist_subcomp0 #_ #a #p1 #p2 #_ wp : (hist (x:a{p2 x})) =
+type hist a = wp:(hist0 a){hist_wp_monotonic wp}
+
+val hist_subcomp0 : #a:Type -> #p1:(a -> Type0) -> #p2:(a -> Type0) -> #_:unit{forall x. p1 x ==> p2 x} -> wp:hist (x:a{p1 x}) ->
+  (hist (x:a{p2 x}))
+let hist_subcomp0 #a #p1 #p2 #_ wp : (hist (x:a{p2 x})) =
   let wp' : hist0 (x:a{p2 x}) = wp in
-  assert (forall (post1:hist_post (x:a{p2 x})) (post2:hist_post (x:a{p2 x})). (hist_post_ord post1 post2 ==> (forall h. wp' post1 h ==> wp' post2 h)));
+  assert (forall h (post1:hist_post h (x:a{p2 x})) (post2:hist_post h (x:a{p2 x})). (hist_post_ord post1 post2 ==>  wp' h post1 ==> wp' h post2));
   assert (hist_wp_monotonic #(x:a{p2 x}) wp');
   wp'
 
-val hist_subcomp : #event_type:Type -> #a:Type -> #p1:(a -> Type0) -> #p2:(a -> Type0) -> wp:hist #event_type (x:a{p1 x}) -> 
-  Pure (hist #event_type (x:a{p2 x})) (requires (forall x. p1 x ==> p2 x)) (ensures (fun _ -> True))
-let hist_subcomp #event_type #a #p1 #p2 wp = hist_subcomp0 #event_type #a #p1 #p2 #() wp
+val hist_subcomp : #a:Type -> #p1:(a -> Type0) -> #p2:(a -> Type0) -> wp:hist (x:a{p1 x}) ->
+  Pure (hist (x:a{p2 x})) (requires (forall x. p1 x ==> p2 x)) (ensures (fun _ -> True))
+let hist_subcomp #a #p1 #p2 wp = hist_subcomp0 #a #p1 #p2 #() wp
 
 
 unfold
-let hist_return (#event_type:Type) (x:'a) : hist #event_type 'a =
-  fun p _ -> p [] x
+let hist_return (x:'a) : hist 'a =
+  admit ();
+  fun _ p -> p [] x
 
 unfold
-let hist_post_shift (#event_type:Type) (p:hist_post #event_type 'a) (lt:list event_type) : hist_post #event_type 'a =
+let hist_post_shift (h:history) (p:hist_post h 'a) (lt:local_trace h) : hist_post (h++lt) 'a =
   fun lt' r -> p (lt @ lt') r
 
 unfold
 let hist_post_bind
   (#a #b:Type)
-  (#event_type:Type)
-  (h:list event_type)
-  (kw : a -> hist #event_type b)
-  (p:hist_post #event_type b) :
-  Tot (hist_post #event_type a) =
+  (h:history)
+  (kw : a -> hist b)
+  (p:hist_post h b) :
+  Tot (hist_post h a) =
   fun lt r ->
-    kw r (hist_post_shift p lt) (List.rev lt @ h)
+    kw r (h ++ lt) (hist_post_shift h p lt)
 
 unfold
-let hist_bind (#event_type:Type) (#a #b:Type) (w : hist #event_type a) (kw : a -> hist #event_type b) : hist #event_type b =
-  fun p h -> w (hist_post_bind #a #b #event_type h kw p) h
+let hist_bind (#a #b:Type) (w : hist a) (kw : a -> hist b) : hist b =
+  fun h p -> w h (hist_post_bind #a #b h kw p)
 
 unfold
-let wp_lift_pure_hist (#event_type:Type) (w : pure_wp 'a) : hist #event_type 'a =
+let wp_lift_pure_hist (w : pure_wp 'a) : hist 'a =
   FStar.Monotonic.Pure.elim_pure_wp_monotonicity_forall ();
-  fun p _ -> w (p [])
+  admit ();
+  fun _ p -> w (p [])
 
-let lemma_wp_lift_pure_hist_implies_as_requires #a #event_type w :
-  Lemma (forall (p:hist_post #event_type a) h. wp_lift_pure_hist w p h ==> as_requires w) =
-    assert (forall (p:hist_post #event_type a) x. p [] x ==> True) ;
+let lemma_wp_lift_pure_hist_implies_as_requires #a w :
+  Lemma (forall h (p:hist_post h a). wp_lift_pure_hist w h p ==> as_requires w) =
+    assert (forall h (p:hist_post h a) x. p [] x ==> True) ;
     FStar.Monotonic.Pure.elim_pure_wp_monotonicity w ;
-    assert (forall (p:hist_post #event_type a). w (fun x -> p [] x) ==> w (fun _ -> True))
+    assert (forall h (p:hist_post h a). w (fun x -> p [] x) ==> w (fun _ -> True))
 
 unfold
-val (⊑) (#event_type:Type) (#a : Type) : hist #event_type a -> hist #event_type a -> Type0
-let (⊑) wp1 wp2 = forall h p. wp2 p h ==> wp1 p h
+val (⊑) (#a : Type) : hist a -> hist a -> Type0
+let (⊑) wp1 wp2 = forall h p. wp2 h p ==> wp1 h p
 
 unfold
-val hist_equiv (#event_type:Type) (#a : Type) : hist #event_type a -> hist #event_type a -> Type0
-let hist_equiv wp1 wp2 = forall h p. wp1 p h <==> wp2 p h
+val hist_equiv (#a : Type) : hist a -> hist a -> Type0
+let hist_equiv wp1 wp2 = forall h p. wp1 h p <==> wp2 h p
 
 unfold
-let hist_if_then_else (wp1 wp2:hist #'event 'a) (b:bool) : hist #'event 'a =
-  fun p h -> (b ==> wp1 p h) /\ ((~b) ==> wp2 p h)
+let hist_if_then_else (wp1 wp2:hist 'a) (b:bool) : hist 'a =
+  fun h p -> (b ==> wp1 h p) /\ ((~b) ==> wp2 h p)
 
 let __list_assoc_l #a (l1 l2 l3 : list a) : Lemma (l1 @ (l2 @ l3) == (l1 @ l2) @ l3) = List.Tot.Properties.append_assoc l1 l2 l3
 let __helper #a (lt lt' : list a) : Lemma (rev_acc lt [] @ rev_acc lt' [] == rev_acc (lt'@lt) []) = List.Tot.Properties.rev_append lt' lt
 let __iff_refl a : Lemma (a <==> a) = ()
 
-let lemma_hist_bind_associativity #a #b #c #ev (w1:hist #ev a) (w2:a -> hist #ev b) (w3: b -> hist #ev c) :
+let lemma_hist_bind_associativity #a #b #c (w1:hist a) (w2:a -> hist b) (w3: b -> hist c) :
   Lemma (hist_bind w1 (fun r1 -> hist_bind (w2 r1) w3) `hist_equiv` hist_bind (hist_bind w1 w2) w3)
   =
   let lhs = hist_bind w1 (fun r1 -> hist_bind (w2 r1) w3) in
   let rhs = hist_bind (hist_bind w1 w2) w3 in
-  let pw (p : hist_post c) (h : list ev) : Lemma (lhs p h <==> rhs p h) =
-    assert (lhs p h <==> rhs p h) by begin
+  let pw (h : history) (p : hist_post h c) : Lemma (lhs h p <==> rhs h p) =
+    assert (lhs h p <==> rhs h p) by begin
       unfold_def (`hist_bind);
       norm [];
       l_to_r [`__list_assoc_l];
@@ -107,17 +109,13 @@ let lemma_hist_bind_associativity #a #b #c #ev (w1:hist #ev a) (w2:a -> hist #ev
     end
   in
   Classical.forall_intro_2 pw
-  
+
 
 unfold
-let to_hist #a #event pre post : hist #event a =
-  fun p h -> pre h /\ (forall lt r. post h r lt ==> p lt r)
+let to_hist #a (pre:hist_pre) (post:(h:history -> a -> local_trace h -> Type0)) : hist a =
+  fun h p -> pre h /\ (forall lt r. post h r lt ==> p lt r)
 
 let post_as_hist = to_hist (fun _ -> True)
 
-(** TODO: is this the trivial wp? **)
-let trivial_hist #a #event : hist #event a =
+let trivial_hist #a : hist a =
   to_hist (fun _ -> True) (fun _ _ _ -> True)
-
-
-type dec_post #event = list event -> list event -> Type0
