rupicola/io/IO.fst
@@ -1,11 +1,11 @@
 module IO
 
 (** we only have bools in STLC right now **)
+open Trace
 
 noeq
 type io (a:Type u#a) : Type u#a =
-| Read : cont:(bool -> io u#a a) -> io a
-| Write : bool -> cont:(unit -> io u#a a) -> io a
+| Call : o:io_ops -> args:io_args o -> (io_res o args -> io a) -> io a
 //| PartialCall : (pre:pure_pre) -> cont:((squash pre) -> io u#a a) -> io a
 | Return : a -> io a
 
@@ -20,27 +20,21 @@ let rec io_bind
   io b =
   match l with
   | Return x -> k x
-  | Read fnc ->
-      Read (fun i ->
-        io_bind #a #b (fnc i) k)
-  | Write x fnc ->
-      Write x (fun i ->
+  | Call o args fnc ->
+      Call o args (fun i ->
         io_bind #a #b (fnc i) k)
 
 let read () : io bool =
-  Read Return
+  Call ORead () Return
 
 let write (x:bool) : io unit =
-  Write x Return
+  Call OWrite x Return
 
-let read_wp () : hist #event bool =
-  to_hist (fun _ -> True) (fun h r lt -> lt == [EvRead r])
+let op_wp (o:io_ops) (args:io_args o) : hist (io_res o args) =
+  to_hist (fun h -> io_pre h o args) (fun h res lt ->
+    io_post h o args res /\ lt == [op_to_ev o args res])
 
-let write_wp (b:bool) : hist #event unit =
-  to_hist (fun _ -> True) (fun h r lt -> lt == [EvWrite b])
-
-let rec theta #a (m:io a) : hist #event a =
+let rec theta #a (m:io a) : hist a =
   match m with
   | Return x -> hist_return x
-  | Read k -> hist_bind (read_wp ()) (fun r -> theta (k r))
-  | Write v k -> hist_bind (write_wp v) (fun r -> theta (k r))
+  | Call o args k -> hist_bind (op_wp o args) (fun r -> theta (k r))
