rupicola/io/Trace.fst
@@ -1,0 +1,80 @@
+module Trace
+
+(**
+  Signature of the operations, and the definition of events
+  and well formed traecs.
+
+  The file should be usable both to define the Dijkstra Monad
+  and the semantics of the Syntactic Language. **)
+
+noeq
+type sig (op:Type u#a) = {
+  args : op -> Type u#a;
+  res : (cmd:op) -> (args cmd) -> Type u#a;
+}
+
+type io_ops = | ORead | OWrite
+
+unfold let io_args (op:io_ops) : Type =
+  match op with
+  | ORead -> unit
+  | OWrite -> bool
+
+unfold let io_res (op:io_ops) (_:io_args op) : Type =
+  match op with
+  | ORead -> option bool
+  | OWrite -> option unit
+
+type event =
+| EvRead  : args:io_args ORead -> io_res ORead args -> event
+| EvWrite : args:io_args OWrite -> io_res OWrite args -> event
+
+let op_to_ev (op:io_ops) (args:io_args op) (res:io_res op args) : event =
+  match op with
+  | ORead -> EvRead args res
+  | OWrite -> EvWrite args res
+
+let destruct_ev (ev:event) : op:io_ops & args:io_args op & io_res op args =
+  match ev with
+  | EvRead a r -> (| ORead, a, r |)
+  | EvWrite a r -> (| OWrite, a, r |)
+
+let trace = list event
+
+unfold
+let io_pre (h:trace) (op:io_ops) (arg:io_args op) : Type0 =
+  match op with
+  | ORead -> True
+  | OWrite -> True
+
+unfold
+let io_post (h:trace) (op:io_ops) (arg:io_args op) (res:io_res op arg) : Type0 =
+  match op with
+  | ORead -> True
+  | OWrite -> True
+
+unfold
+let test_event (h:trace) (ev:event) =
+  match ev with
+  | EvRead v r -> io_pre h ORead v /\ io_post h ORead v r
+  | EvWrite v r -> io_pre h OWrite v /\ io_post h OWrite v r
+
+let rec well_formed_local_trace (h:trace) (lt:trace) : Tot Type0 (decreases lt) =
+  match lt with
+  | [] -> True
+  | ev :: tl -> test_event h ev /\ well_formed_local_trace (ev::h) tl
+
+type history = trace (** a history is a trace kept backwards **)
+
+type local_trace (h:trace) =
+  lt:trace{well_formed_local_trace h lt}
+
+open FStar.List.Tot
+
+let (++) (h:history) (lt:local_trace h) : history =
+  List.rev lt @ h
+
+let trans_well_formed_local_trace (h:trace) (lt:local_trace h) (lt1:local_trace (h++lt)) :
+  Lemma (well_formed_local_trace h (lt @ lt1))
+  [SMTPat (well_formed_local_trace h (lt @ lt1))] =
+    admit ()
